Impl/ImplFlushPolicy.i.dfy
@@ -56,9 +56,9 @@ module ImplFlushPolicy {
   function method TotalCacheSize(s: ImplVariables) : (res : uint64)
   reads s, s.cache, s.cache.Repr
   requires s.cache.Inv()
-  requires |s.cache.I()| + |s.outstandingBlockReads| < 0x1_0000_0000_0000_0000
+  requires |s.cache.I()| + s.outstandingBlockReads.Count as int < 0x1_0000_0000_0000_0000
   {
-    s.cache.Count() + (|s.outstandingBlockReads| as uint64)
+    s.cache.Count() + s.outstandingBlockReads.Count
   }
 
   method getActionToSplit(k: ImplConstants, s: ImplVariables, stack: seq<BT.G.Reference>, slots: seq<uint64>, i: uint64) returns (action : ImplModelFlushPolicy.Action)
